clean up and comments

Lerchner/DFA_to_RegExp.thy
@@ -1,149 +1,338 @@
 theory DFA_to_RegExp
 
-imports 
-"$AFP/Regular-Sets/Regular_Exp"   
+imports "DFA_Locale_simple"
 begin
 
+(** 
+  This theory file contains the proof of the conversion of a (simplified) DFA to a regular expression.
+  The proof is based on the book "Introduction to Automata Theory, Languages, and Computation" by John E. Hopcroft, Rajeev Motwani, and Jeffrey D. Ullman.
 
-(** See proof of theorem 3.4 in **)
-(**https://www-2.dc.uba.ar/staff/becher/Hopcroft-Motwani-Ullman-2001.pdf**)
-
-locale dfa =
-  fixes n :: nat
-  and sigma :: "'a list"
-  and nxt :: "nat \<Rightarrow> 'a \<Rightarrow> nat"
-  (* initial state is 1 *)
-  and Fin :: "nat set"
-  assumes all_states_greater_than_0: "(\<forall>s . s \<in> Fin \<longrightarrow> s > 0) \<and> (\<forall>i a . nxt i a  > 0)"
-begin
-
-fun nxts :: "'a list \<Rightarrow> nat \<Rightarrow> nat" where
-  "nxts [] q = q" |
-  "nxts (a#w) q = nxts w (nxt q a)"
-  
-definition accepted :: "'a list \<Rightarrow> bool" where
-  "accepted w = (nxts w 1 \<in> Fin)"
-  
-(* Your work goes here: *)
-
-type_synonym 'b path = "nat * ('b list) * nat"
-
-definition path_valid :: "'a path \<Rightarrow> bool" where
-  "path_valid p \<longleftrightarrow> (let (i,w,j) = p in  (nxts w i = j))"
-
-fun states_visited :: "'a path \<Rightarrow> nat list" where
-  "states_visited (i, [], j) = []" | 
-  "states_visited (i, a#w, j) = 
-     (let next = nxt i a in 
-      if next = j then [] 
-      else next # states_visited (next, w, j))"
-
-lemma states_visited_gt_0: "x \<in> set (states_visited (i,w,j)) \<Longrightarrow> x >0 "
-  apply(induction w arbitrary:i)
-  apply(auto)
-  by (smt (verit, ccfv_threshold) all_states_greater_than_0 length_pos_if_in_set less_numeral_extra(3) list.size(3) set_ConsD)
-
-lemma states_visited_valid:
-  assumes "path_valid (i,w,j)"
-  shows " (\<exists>xs ys. nxts xs i = k \<and> xs @ ys = w \<and> xs \<noteq> [] \<and> ys \<noteq> []) \<longleftrightarrow> k \<in> set (states_visited (i,w,j)) "
-  sorry
-
-definition path_restricted :: " 'a path \<Rightarrow> nat \<Rightarrow> bool" where
-  "path_restricted p k \<longleftrightarrow> (path_valid p \<and> (\<forall>s. s \<in> set (states_visited p) \<longrightarrow> s \<le> k))"
+  The proof is based on the theorem 3.4 in the book.
+  https://www-2.dc.uba.ar/staff/becher/Hopcroft-Motwani-Ullman-2001.pdf
+**)
 
 
+(** 
+  I was able to prove correctness of the base case of the conversion function R i j 0, 
+  and completed half of the induction step R i j (k+1).
+
+  I got stuck in the induction step, because I could not get the claimed decomposition lemma to work.
+  But i think there is not much missing to complete the proof.
+**)
 
 
-fun path_goes_through_node :: "'a path \<Rightarrow> nat \<Rightarrow> bool" where
-  "path_goes_through_node p k = (k \<in> set (states_visited p))"
+context dfa begin
 
- 
-fun rexp_goes_through_node :: "'a rexp \<Rightarrow> nat \<Rightarrow> bool" where
-  "rexp_goes_through_node rexp k = (\<exists>w \<in> lang rexp. path_goes_through_node (1, w, nxts w 1) k) "
+section "Defintion of the conversion function R i j k"
 
 
- (** todo  missing case y**)
-lemma split_path_at_node:"p = (i, w, j) \<Longrightarrow> path_valid p \<Longrightarrow>  path_goes_through_node p k \<Longrightarrow> \<exists> x y z . (x @ y @ z = w \<and>
-                                                                        \<not> path_goes_through_node (i, x, k) k \<and>
-                                                                        \<not> path_goes_through_node (k, u, j) k)"
-  sorry
-
-
+(** 
+  The function arcs_rexp i j generates a regular expression 
+  generating all single letter paths from state i to state j.
+**)
 definition arcs_rexp :: "nat \<Rightarrow> nat \<Rightarrow> 'a rexp" where
-  "arcs_rexp i j =  List.foldr Plus 
-                  (List.map Atom [ a \<leftarrow> sigma. nxt i a = j]) 
-              Zero"
+   "arcs_rexp i j = foldr Plus [Atom a . a \<leftarrow> sigma, nxt i a = j] Zero"
 
-lemma lang_foldr:"lang (List.foldr Plus xs Zero) = \<Union>{lang x | x. x \<in> set xs} "
-proof(induction xs)
-  case Nil
-  then show ?case by simp
-next
-  case (Cons a xs)
-
- have "\<Union> {lang x |x. x \<in> set (a # xs)} = \<Union> {lang x |x. x \<in> (set xs \<union>  {a})} "
-   by auto
-  also have "... = \<Union> {lang x |x. x \<in> (set xs )} \<union> lang a"
-    by blast
-  then show ?case
-    by (simp add: local.Cons sup_commute) 
+lemma lang_arcs_rexp:" lang (arcs_rexp i j) = { [a] | a. a \<in> set sigma \<and>  nxt i a = j}"
+proof -
+    have " lang (arcs_rexp i j) = lang (foldr Plus [Atom a . a \<leftarrow> sigma, nxt i a = j] Zero)"
+      by (simp add: arcs_rexp_def)
+    also have "... = \<Union>{lang x | x. x \<in> set [Atom a . a \<leftarrow> sigma, nxt i a = j]}"
+      using lang_combine_plus by blast
+    also have "... = \<Union>{lang x | x. x \<in> {Atom a | a. a \<in> set sigma \<and> nxt i a = j}}"
+      by auto
+    also have "... = \<Union>{ lang (Atom a) | a. a \<in> set sigma \<and> nxt i a = j}"
+      by blast
+    also have "... =  { [a] | a. a \<in> set sigma \<and> nxt i a = j}"
+      by(auto)
+    finally show ?thesis 
+      by auto
 qed
 
+(**
+  The conversion function R i j k should generate a regular expression
+  corresponding to the set of words that represent a path from state i to state j, only using states from S up to state k.
+**)
+fun R :: "nat \<Rightarrow> nat \<Rightarrow> nat \<Rightarrow> 'a rexp " where
+  "R i j 0 = (if i \<notin> S \<or> j \<notin> S then Zero else 
+               (if i \<noteq> j then arcs_rexp i j else Plus One (arcs_rexp i j)))" |
+  "R i j (Suc k) = (if i \<notin> S \<or> j \<notin> S then Zero else 
+                   (  let R'= R    i       j    k in
+                      let u = R    i    (Suc k) k in
+                      let v = R (Suc k) (Suc k) k in
+                      let w = R (Suc k)    j    k in
+                    Plus  R' (Times u (Times (Star v) w))))"
 
-lemma arcs_lang:"[a] \<in> lang (arcs_rexp i j) \<longleftrightarrow>  nxt i a = j "
-  unfolding arcs_rexp_def
+
+
+section "Proofs about the conversion function R i j k"
+
+
+
+
+
+
+
+subsection "Proofs about the base case R i j 0"
+
+lemma lang_base_case:"lang (R i j 0) = (if i\<notin> S \<or> j \<notin> S then {} 
+                                   else { [a] | a. a \<in> set sigma \<and>  nxt i a = j}  \<union> (if i = j then {[]} else {}))"
+   by (simp add: lang_arcs_rexp)
+
+
+
+lemma R_valid_path:"w\<in> lang (R i j k) \<Longrightarrow> i \<in> S \<and> j \<in> S"
+  apply(induction i j k rule:R.induct)
+  apply (metis empty_iff lang_base_case)
+  apply(auto)
+  apply (smt (verit, ccfv_threshold) empty_iff lang.simps(1))
+  by (smt (verit, best) all_not_in_conv lang.simps(1))
+
+
+(** 
+  First direction:
+  If a word w is in the language of R i j 0, then w is a path from i to j and its intermediate path is restricted to 0.
+**)
+lemma langRij0_1:
+  assumes "w \<in> lang (R i j 0)"
+  shows "(word_run_from_i_j w i j \<and>  intermediate_path_restricted (path_of_word w i) 0)"
+ proof -
+   have lang:"lang (R i j 0) =  { [a] | a. a \<in> set sigma \<and>  nxt i a = j}  \<union> (if i = j then {[]} else {})"
+     by (metis (no_types, lifting) assms lang_base_case R_valid_path)
+
+   have " i \<in> S "
+     using assms R_valid_path by blast
+
+   then have "word_run_from_i_j w i j"
+     apply(cases "i = j")
+     using lang assms word_run_from_i_j_def by force +
+
+   have "w \<in> { [a] | a. a \<in> set sigma \<and>  nxt i a = j}  \<union> (if i = j then {[]} else {})"
+      by (metis (no_types, lifting) lang_base_case R_valid_path assms)
+
+    then  have "path_of_word w i = (if w=[] then [i] else [i,j])"
+      by(cases "i=j") auto
+ 
+    then  have "intermediate_path (path_of_word w i) = [] "
+     using assms by force
+
+   then have "intermediate_path_restricted (path_of_word w i) 0"
+     unfolding intermediate_path_restricted_def
+     by simp
+  
+   then show ?thesis
+     by (simp add: \<open>word_run_from_i_j w i j\<close>)
+ qed
+
+(** 
+  Second direction:
+  If a word w is a path from i to j and its intermediate path is restricted to 0, then w is in the language of R i j 0.
+**)
+lemma langRij0_2:
+  assumes "word_run_from_i_j w i j" and "intermediate_path_restricted (path_of_word w i) 0"
+  shows "w \<in> lang (R i j 0)"
+using assms proof -
+   have "intermediate_path (path_of_word w i) = []"
+     using assms(1) assms(2) no_intermediate_path_k0 word_run_sound by blast
+ 
+  then have "path_of_word w i  =(if w=[] then [i] else [i,nxt i (hd w)])"
+    using assms path_shape_no_intermediate by auto
+
+  then have "w = (if w=[] then [] else [hd w])"
+    by (metis list.distinct(1) list.inject list.sel(1) path_of_word.elims)
+
+  then consider "w=[]" | "w=[hd w]"
+    by meson
+  then show "w \<in> lang (R i j 0)"
+    apply(cases)
+    using assms(1) word_run_from_i_j_def apply fastforce
+    apply(auto simp add:lang_base_case lang_arcs_rexp)
+    using assms word_run_from_i_j_def intermediate_path_restricted_def apply auto
+    using word_run_sound apply blast
+    by (metis in_mono list.set_intros(1) nxts.simps(1) nxts.simps(2)) +
+qed
+
+(** 
+  The language of R i j 0 is the set of words that represent a path from i to j, only using states from S up to state 0.
+**)
+corollary langRij0_correct: "i \<in> S \<Longrightarrow> j \<in> S \<Longrightarrow> w \<in> lang (R i j 0) \<longleftrightarrow>   word_run_from_i_j w i j \<and> intermediate_path_restricted (path_of_word w i) 0"
+  using langRij0_1 langRij0_2 by blast
+
+
+
+
+
+
+
+
+
+
+
+subsection "Proofs about the induction step R i j (k+1)"
+
+(** 
+I cant get the following decomposition lemma to work / be sound. The proof in the book claims that it should work somehow like this. But nitpick, and metis are unhappy with it.
+**)
+
+(**
+lemma word_decomposition:"(word_run_from_i_j w i j \<Longrightarrow> intermediate_path_restricted (path_of_word w i) k \<Longrightarrow> k>0 \<Longrightarrow>  k \<in> set( (path_of_word w i))) \<Longrightarrow> 
+                                                                         (\<exists> w1 wss w3. w = w1 @ (concat ( wss)) @ w3 
+                                                                          \<and>                word_run_from_i_j  w1 i k \<and>  k \<notin> set(intermediate_path (path_of_word w1 i))
+                                                                          \<and> (\<forall>p \<in> set wss. word_run_from_i_j  p  k k \<and>  k \<notin> set(intermediate_path (path_of_word p  k)))
+                                                                          \<and>                word_run_from_i_j  w3 k j \<and>  k \<notin> set(intermediate_path (path_of_word w3 k))
+                                                                          )"
+ 
   sorry
+**)
+ 
 
-(** todo start at -1?**)
-fun R:: "nat \<Rightarrow> nat \<Rightarrow> nat \<Rightarrow> 'a rexp " where
-  "R i j 0 = (if i \<noteq> j then arcs_rexp i j else Plus Zero (arcs_rexp i j))" |
-  "R i j (Suc k) = (let R' = R i j k in
-                           if \<not>rexp_goes_through_node R' k then 
-                              R'
-                           else
-                              let u = R    i    (Suc k) k in
-                              let v = R (Suc k) (Suc k) k in
-                              let w = R (Suc k)    j    k in
-                              Plus  R' (Times u (Times (Star v) w)))"
+lemma Rmono: "lang (R i j k) \<subseteq> lang (R i j (k + 1))"
+  apply(induction  i j k rule:R.induct)
+   apply(auto)
+  done
 
-
-
-
-
-
-lemma " path_restricted (i, w, j) k \<Longrightarrow> w \<in> lang (R i j k)"
-proof(induction k arbitrary: i j)
+lemma langRijk: 
+  assumes " k\<le>n "
+  shows " w \<in> lang (R i j k) \<longleftrightarrow> (word_run_from_i_j w i j \<and>  intermediate_path_restricted (path_of_word w i) k)"
+using assms proof(induction k arbitrary: i j w)
   case 0
-
-  then  show ?case 
-
-  proof(cases "i=j")
-    case True
-    then show ?thesis 
-      unfolding path_restricted_def path_valid_def 
-      apply(auto)
-      sorry
-  next
-    case False
-    then show ?thesis sorry
-  qed
+  then show ?case
+    using langRij0_1 langRij0_2 by blast  
+   
 next
   case (Suc k)
-  then show ?case sorry
-qed
+
+  let ?R'= "R i j k" 
+ 
+  show ?case 
+  proof(cases "\<forall> x \<in> set (intermediate_path (path_of_word  w i)) . x < k+1")
+    case not_through_k_plus_one:True
+
+    have "w \<in> lang ?R' \<longleftrightarrow> (word_run_from_i_j w i j \<and> intermediate_path_restricted (path_of_word w i) (Suc k))"
+    proof(rule iffI)
+      assume "w \<in> lang ?R'"
+ 
+      show "(word_run_from_i_j w i j \<and> intermediate_path_restricted (path_of_word w i) (Suc k))"
+        by (meson Suc.IH Suc.prems Suc_leD \<open>w \<in> lang (R i j k)\<close> intermediate_path_restricted_def le_SucI)
+    next
+      assume "(word_run_from_i_j w i j \<and> intermediate_path_restricted (path_of_word w i) (Suc k))"
+
+      then have "intermediate_path_restricted (path_of_word w i) k"
+        unfolding intermediate_path_restricted_def
+        using not_through_k_plus_one le_Suc_eq by fastforce
+       
+      then  show "w \<in> lang ?R'"
+        by (simp add: Suc.IH Suc.prems Suc_leD \<open>word_run_from_i_j w i j \<and> intermediate_path_restricted (path_of_word w i) (Suc k)\<close>) 
+    qed
+
+    have "(w \<in> lang (R i j (Suc k))) \<Longrightarrow> (word_run_from_i_j w i j \<and> intermediate_path_restricted (path_of_word w i) (Suc k))"
+    proof -
+      assume "(w \<in> lang (R i j (Suc k)))"
+      then show ?thesis
+      proof(cases "(w \<in> lang (R i j k))")
+        case True
+        then show ?thesis
+          by (simp add: \<open>(w \<in> lang (R i j k)) = (word_run_from_i_j w i j \<and> intermediate_path_restricted (path_of_word w i) (Suc k))\<close>) 
+      next
+        case False
+        let ?u = "R    i    (Suc k) k "
+        let ?v = "R (Suc k) (Suc k) k" 
+        let ?w = "R (Suc k)    j    k" 
+
+       
+
+         have lang_times:"w \<in> lang (Times (R a b k) (R b c k)) \<Longrightarrow> word_run_from_i_j w a c" for a b c w
+          using Suc.IH Suc.prems word_run_trans by fastforce
+        
+          have word_run_star:"a \<in> S \<Longrightarrow> w \<in> star (lang (R a a k)) \<Longrightarrow>  word_run_from_i_j w a a" for a w
+          proof -
+            assume "a \<in> S"
+            show "w \<in> star (lang (R a a k)) \<Longrightarrow> word_run_from_i_j w a a"
+              apply(induction rule:star_induct)
+              apply (simp add: \<open>a \<in> S\<close> word_run_from_i_j_def)
+              using Suc.IH Suc.prems Suc_leD word_run_trans by blast
+          qed
+          
+          have "w \<in> lang (Plus  ?R' (Times ?u (Times (Star ?v) ?w)))"
+           by (metis R.simps(2) R_valid_path \<open>w \<in> lang (R i j (Suc k))\<close>)
+          then have "word_run_from_i_j w i j"
+            using lang_times word_run_star apply (simp add: False)
+            by (smt (verit, best) R_valid_path Suc.IH Suc.prems Suc_leD concE word_run_trans)
+
+ 
+        then show ?thesis
+          by (metis Suc_eq_plus1 intermediate_path_restricted_def less_or_eq_imp_le not_through_k_plus_one)
+      qed
+    qed
+
+   then show ?thesis
+     by (metis Rmono Suc_eq_plus1 \<open>(w \<in> lang (R i j k)) = (word_run_from_i_j w i j \<and> intermediate_path_restricted (path_of_word w i) (Suc k))\<close> subset_iff)  
+           
+  next
+    case False
+
+    (**
+    I got stuck here, because I cant get the decomposition lemma to work.
+    **)
+ 
+     then show ?thesis
+       sorry
+
+   qed
+ qed
 
 
-  
+
+(** 
+  The language of R i j k is the set of words that represent a path from i to j, only using states from S up to state k.
+**)
+corollary langRijk_correct: "i \<in> S \<Longrightarrow> j \<in> S \<Longrightarrow> w \<in> lang (R i j n) \<longleftrightarrow>   word_run_from_i_j w i j"
+  using langRijk restricted_n by auto
+
+
+
+
+
+
+
+section "Proofs about the final conversion function rexp_of"
+
+
+(** 
+  To create the final regular expression, we combine all regular expressions from the start state (1) to all final states (Fin).
+**)
 definition rexp_of :: "'a rexp" where
 "rexp_of = List.foldr Plus 
-             [ R 0 j n . j \<leftarrow> sorted_list_of_set Fin]
+             [ R 1 f n . f \<leftarrow> sorted_list_of_set Fin]
            Zero"
 
-theorem "w \<in> lang (rexp_of) \<longleftrightarrow> accepted w"
-  sorry
+(** 
+  The language of the created regular expression is the set of all accepted words.
+**)
+theorem rexp_of_correct: "w \<in> lang (rexp_of) \<longleftrightarrow> accepted w"
+proof -
+  have f:"finite S"
+    by (simp add: state_set_def)
+
+  have "lang (rexp_of) = \<Union>{lang x | x. x \<in> set [ R 1 j n . j \<leftarrow> sorted_list_of_set Fin]}"
+    by (simp add: lang_combine_plus rexp_of_def)
+  also have "... = \<Union>{lang (R 1 j n) | j. j \<in> Fin} "
+    using f finite_subset states_subset by fastforce
+  also have "... = {w.  (\<exists>j \<in> Fin. w \<in> lang (R 1 j n))  }"
+    by blast
+   also have "... = {w.  (\<exists>j \<in> Fin. word_run_from_i_j w 1 j)  }"
+     by (metis in_mono start_exist states_subset langRijk_correct)
+   also have "... = {w.  (\<exists>j \<in> Fin.  set w \<subseteq> set sigma \<and> nxts w 1 = j)  }"
+     using start_exist word_run_from_i_j_def by auto
+   also have "...= {w. accepted w }"
+     using accepted_def by auto
+  ultimately show ?thesis
+    by simp
+qed
+
+corollary "{w. accepted w} = lang (rexp_of)"
+  using rexp_of_correct by auto
 
 end
-
-
 
 end
